---
title: "The Triangle of Power"
categories: [notation, latex]
image: "penrose.png"
jupyter: python3
---

A post on Math Overflow about the relationship between powers, roots, and logs sparked the birth of a notation to harmonize these seemingly unrelated concepts. Grant Sanderson from 3Blue1Brown further popularized and named this notation as, "The Triangle of Power"

# Exponents, Logs, and Roots

There are three general ways to describe the following mathematical equality: $$
\begin{gather*}
\underbrace{\text{  }2 \times 2 \times 2}_\text{3} = 8 \\
\textit{(2 multiplied by itself 3 times equals 8)}
\end{gather*}
$$

-   **2** multiplied by itself **3** times equals *what*? (answer is 8)
-   *what* multiplied by itself **3** times equals **8**? (answer is 2)
-   multiply **2** by itself *how many times* to equal **8**? (answer is 3)

or in matematical notation:

-   **Exponents** $2^3=8$
-   **Logarithms** $\sqrt[3]8=2$
-   **Roots** $\log_2(8) = 3$

It is unfortunate that all three of these relationships use different notation types to represent the same truism that $2\times2\times2=8$. Various websites and media have explored alternative ways to represent this relationship. The one explored in this article is the **Triangle of Power**.

# The Triangle of Power... $_{a}\stackrel{b}\triangle _{c}$

Take the equation, $2\times2\times2=8$. Using new notation, I will represent this relationship in a triad as so:

$$
\begin{align*}
& _{2}\stackrel{3}\triangle _{8} 
\end{align*}
$$

This means that I can represent each individual description (exponents, logs, and roots) as so:

$$
\begin{align*}
& 2^3 = 8 & \Leftrightarrow {} \stackrel{3}{_2\triangle_{\phantom{c}}} = 8 \\
& \sqrt[3]{8} = 2 & \Leftrightarrow {} \stackrel{3}{_\phantom{a}\triangle_{8}} = 2\\
& \log_2\left(8\right) = 3 & \Leftrightarrow {} \stackrel{}{_2\triangle_{8}} = 3\\
\end{align*}
$$

We can use this new notation with the variables $a$, $b$, and $c$ to make this relationship more general. $$
\begin{align*}
& a^b = c & \Leftrightarrow {} \stackrel{b}{_a\triangle_{\phantom{c}}} = c \\
& \sqrt[b]{c} = a & \Leftrightarrow {} \stackrel{b}{_\phantom{a}\triangle_{c}} = a\\
& \log_a\left(c\right) = b & \Leftrightarrow {} \stackrel{}{_a\triangle_{c}} = b
\end{align*}
$$

# Properties of these operators (in standard notation)

## $a$ remains constant

$$
\begin{align*}
&\text{Properties of Logarithms}
&\text{Properties of Exponents}
\\\\
&
\log_a(x\times y) = \log_a(x) + \log_b(x)
&
a^{x + y} = a^x \times a ^y
\\\\
&
\log_a(\frac{x}{y}) = \log_a(x) - \log_b(x)
&
a^{x - y} = \frac{a^x}{a^y}
\end{align*}
$$

## $b$ remains constant

$$
\begin{align*}
&\text{Properties of Exponents}
&\text{Properties of Roots}
\\\\
&   xy^b = x^b \times y^b
&   \sqrt[b]{x\times y} = \sqrt[b]{x} \times \sqrt[b]{y}
\\\\
&   \left(\frac{x}{y}\right)^b = \frac{x^b}{y^b}
&   \sqrt[b]{\frac{x}{y}} = \frac{\sqrt[b]{x}}{\sqrt[b]{y}}
\end{align*}
$$

## $c$ remains constant

$$
\begin{align*}
&\text{Properties of Logarithms}
&\text{Properties of Roots}
\\\\
&   \log_{x\times y}(c) = \left(\left(\log_xc\right)^{-1} + \left(\log_yc\right)^{-1}\right)^{-1}
&   \sqrt[(x^{-1}+ y^{-1})^{-1}]{c} = \sqrt[x]{c} \times \sqrt[y]{c}
\\\\
&   \log_{\frac{x}{y}}(c) = \left(\left(\log_xc\right)^{-1} - \left(\log_yc\right)^{-1}\right)^{-1}
&   \sqrt[(x^{-1}- y^{-1})^{-1}]{c} = \frac{\sqrt[x]{c}}{\sqrt[y]{c}}
\end{align*}
$$

# Properties of these operators (in power triangle notation)

## $a$ remains constant

$$
\begin{align*}
&\text{Properties of Logarithms}
&\text{Properties of Exponents}
\\\\
&
_{a}
\stackrel{\phantom{b}}
\triangle _{xy} 
={}
_{a}\stackrel{\phantom{b}}\triangle _{x} +{}
_{a}\stackrel{\phantom{b}}\triangle _{y}
&
_{a}
\stackrel{x+y}
\triangle _{\phantom{c}} 
={}
_{a}\stackrel{x}\triangle _{\phantom{c}} \times{}
_{a}\stackrel{y}\triangle _{\phantom{c}}
\\\\
&_{a}
\stackrel{\phantom{b}}
\triangle _{\frac{x}{y}} 
={}
_{a}\stackrel{\phantom{b}}\triangle _{x} -{}
_{a}\stackrel{\phantom{b}}\triangle _{y}
&
_{a}
\stackrel{x-y}
\triangle _{\phantom{c}} 
={}
\frac
{_{a}\stackrel{x}\triangle _{\phantom{c}}}
{_{a}\stackrel{y}\triangle _{\phantom{c}}}
\end{align*}
$$

## $b$ remains constant

$$
\begin{align*}
&\text{Properties of Exponents}
&\text{Properties of Roots}
\\\\
&
_{x\times y}
\stackrel{b}
\triangle _{\phantom{c}} 
={}
_{x}\stackrel{b}\triangle _{} \times{}
_{y}\stackrel{b}\triangle _{}
&
_{\phantom{a}}
\stackrel{b}
\triangle _{x\times y} 
={}
_{\phantom{x}}\stackrel{b}\triangle _{x} \times{}
_{\phantom{x}}\stackrel{b}\triangle _{y}
\\\\
&_{\frac{x}{y}}
\stackrel{b}
\triangle _{\phantom{c}} 
={}
\frac
{_{x}\stackrel{b}\triangle _{\phantom{c}} }
{_{y}\stackrel{b}\triangle _{\phantom{c}} }
&
_{\phantom{a}}
\stackrel{b}
\triangle _{\frac{x}{y}} 
=
\frac
{_{\phantom{a}}\stackrel{b}\triangle _{x}}
{_{\phantom{a}}\stackrel{b}\triangle _{y}}
\end{align*}
$$

## $c$ remains constant

$$
\begin{align*}
&\text{Properties of Logarithms}
&\text{Properties of Roots}
\\\\
&
_{x\times y}
\stackrel{\phantom{b}}
\triangle _{c} 
={}
\left(
\left( _{x}\stackrel{}\triangle _{c}\right)^{-1} +{}
\left(_{y}\stackrel{}\triangle _{c}\right)^{-1}
\right)^{-1}
&
_{\phantom{a}}
\stackrel{
  \left(x^{-1}+y^{-1}\right)^{-1}
}
\triangle _{c} 
={}
_{\phantom{x}}\stackrel{x}\triangle _{c} \times{}
_{\phantom{x}}\stackrel{y}\triangle _{c}
\\\\
&
_{\frac{x}{y}}
\stackrel{\phantom{b}}
\triangle _{c} 
={}
\left(
\left( _{x}\stackrel{}\triangle _{c}\right)^{-1} -{}
\left(_{y}\stackrel{}\triangle _{c}\right)^{-1}
\right)^{-1}
&
_{\phantom{a}}
\stackrel{
  \left(x^{-1}-y^{-1}\right)^{-1}
}
\triangle _{c} 
={}
\frac
{_{\phantom{x}}\stackrel{x}\triangle _{c} }
{_{\phantom{x}}\stackrel{y}\triangle _{c}}
\end{align*}
$$

# Inverse identities

Inverse identities: $a = f(f^{-1}(a))$ - are as follows below:

$$
\begin{align*}
a &= \sqrt[b]{a^b} &=\sqrt[log_a(c)]{c}
\\\\
b &= \log_a(a^b) &=\log_{\sqrt[a]{c}}(c)
\\\\
c &= (\sqrt[b]{c})^c &=a^{\log_a(c)}
\\\\
\end{align*}
$$

Inverse identities in triangle notation are as follows below:

$$
\begin{align*}
a &= \text{ }
_{\phantom{a}}
\stackrel{b}
\triangle _{    _{a}\stackrel{b}\triangle _{\phantom{c}}    } 
\text{ } &= \text{ }
_{\phantom{a}}
\stackrel{_{a}\stackrel{\phantom{b}}\triangle _{c}}
\triangle _{c} \\\\
b &= \text{ }
_{    _{\phantom{a}}\stackrel{b}\triangle _{c}    }
\stackrel{\phantom{b}}
\triangle _{c} 
\text{ } &= \text{ }
_{a}
\stackrel{\phantom{b}}
\triangle _{    _{a}\stackrel{b}\triangle _{\phantom{c}}    } \\\\ 
c &= \text{ }
_{    _{\phantom{a}}\stackrel{b}\triangle _{c}    }
\stackrel{b}
\triangle _{\phantom{c}} 
\text{ } &= \text{ }
_{a}
\stackrel{    _{a}\stackrel{\phantom{b}}\triangle _{c}    }
\triangle _{\phantom{c}} \\\\
\end{align*}
$$
